# Derivatives
Note: these will also include proofs
## Derivative definition
$\lim_{h \to 0}\frac{f(x+h)-f(x)}{h}$
### Proof: Differentiability implies continuity
## Constant rule
$\frac{d}{dx}(c) = 0$
## Constant multiple rule
$\frac{d}{dx}(c*f(x)) = c*\frac{d}{dx}(f(x))$
## Sum/Difference rule
$\frac{d}{dx}(f(x)\pm g(x)) = \frac{d}{dx}f(x)\pm\frac{d}{dx}g(x)$
## Chain rule
$\frac{dy}{dx} = \frac{dy}{du}*\frac{du}{dx}$
## sin(x), cos(x)
$\frac{d}{dx}sin(x) = cos(x)$

$\frac{d}{dx}cos(x) = -sin(x)$
## $e^x$
$\frac{d}{dx}e^x= e^x$
## ln(x)
$\frac{d}{dx}ln(x)= \frac{1}{x}$

Proof: Go to "Implicit differentiation"
## Product/Quotient rule
$\frac{d}{dx}(u*v) = v * \frac{d}{dx}u+u * \frac{d}{dx}v$

$\frac{d}{dx}(\frac{u}{v}) = \frac{v*\frac{du}{dx}-u*\frac{dv}{dx}}{v^2}$
## tan(x), cot(x), sec(x), cosec(x)
$\frac{d}{dx}tan(x) = sec^2(x)$

$\frac{d}{dx}cot(x) = -cosec^2(x)$

$\frac{d}{dx}sec(x) = tan(x)sec(x)$

$\frac{d}{dx}cosec(x) = -cot(x)cosec(x)$
## Chain rule
$\frac{dy}{dx} = \frac{dy}{du} * \frac{du}{dx}$
### Exponentials
$\frac{d}{dx}C^x = ln(C) * C^x$

Proof:

$C^x = e^{ln(C)x}$

Chain rule

$u=ln(C)x$

$y = e^u$

$\frac{dy}{dx} = \frac{dy}{du} * \frac{du}{dx} = e^u * ln(C)$

$\frac{d}{dx}C^x = ln(C) * C^x$
## Implicit differentiation
## Inverse functions
### Inverse trigs



